proofs/transform/FullSubstitution.v
@@ -1,0 +1,447 @@
+(*Here, we define the full substitution of terms for variables
+  and (TODO) terms for terms*)
+(*TODO: maybe move this to Substitution.v, but only used for
+  transformations*)
+
+Require Import Denotational.
+Set Bullet Behavior "Strict Subproofs".
+
+(*t2[t1/x]*)
+Fixpoint sub_t (t1: term) (x: vsymbol) (t2: term) : term :=
+  match t2 with
+  | Tconst c => Tconst c
+  | Tvar v  => 
+    (*The base case*)
+    if vsymbol_eq_dec x v then t1 else Tvar v
+  | Tfun fs tys tms =>
+    Tfun fs tys (map (sub_t t1 x) tms)
+  | Tlet tm1 v tm2 =>
+    Tlet (sub_t t1 x tm1) v
+    (if vsymbol_eq_dec x v then tm2 else (sub_t t1 x tm2))
+  | Tif f1 tm1 tm2 =>
+    Tif (sub_f t1 x f1) (sub_t t1 x tm1) (sub_t t1 x tm2)
+  | Tmatch tm ty ps =>
+    Tmatch (sub_t t1 x tm) ty
+    (map (fun p => if in_bool vsymbol_eq_dec x (pat_fv (fst p)) then
+      p else (fst p, sub_t t1 x (snd p))) ps)
+  | Teps f1 v =>
+    if vsymbol_eq_dec x v then t2 else
+    Teps (sub_f t1 x f1) v
+  end
+with sub_f (t1: term) (x: vsymbol) (f: formula) : formula :=
+  match f with
+  | Fpred p tys tms => Fpred p tys (map (sub_t t1 x) tms)
+  | Fquant q v f' =>
+    if vsymbol_eq_dec x v then f else
+    Fquant q v (sub_f t1 x f')
+  | Feq ty tm1 tm2 =>
+    Feq ty (sub_t t1 x tm1) (sub_t t1 x tm2)
+  | Fbinop b f1 f2 =>
+    Fbinop b (sub_f t1 x f1) (sub_f t1 x f2)
+  | Fnot f' => Fnot (sub_f t1 x f')
+  | Ftrue => Ftrue
+  | Ffalse => Ffalse
+  | Flet tm v f' =>
+    Flet (sub_t t1 x tm) v 
+      (if vsymbol_eq_dec x v then f' else
+      sub_f t1 x f')
+  | Fif f1 f2 f3 =>
+    Fif (sub_f t1 x f1) (sub_f t1 x f2) (sub_f t1 x f3)
+  | Fmatch tm ty ps =>
+    Fmatch (sub_t t1 x tm) ty
+      (map (fun p => if in_bool vsymbol_eq_dec x (pat_fv (fst p)) then
+        p else (fst p, sub_f t1 x (snd p))) ps)
+  end.
+
+  (*t[y/x]*)
+(*Definition vsub_t (x y: vsymbol) (t: term) : term :=
+  sub_t (Tvar y) x t.
+Definition vsub_f (x y: vsymbol) (f: formula) : formula :=
+  sub_f (Tvar y) x f.*)
+(*This is a generalized version of [sub_var_t] and [sub_var_f]*)
+Lemma sub_var_equiv (t: term) (f: formula) :
+  (forall (x y: vsymbol), 
+    sub_var_t x y t = sub_t (Tvar y) x t) /\
+  (forall (x y: vsymbol),
+    sub_var_f x y f = sub_f (Tvar y) x f).
+Proof.
+  revert t f; apply term_formula_ind; simpl; auto; intros;
+  try solve[rewrite H; auto];
+  try solve[rewrite H, H0; auto];
+  try solve[rewrite H, H0, H1; auto].
+  - vsym_eq x v.
+  - f_equal. induction l1; simpl; auto.
+    inversion H; subst; auto. f_equal; auto.
+  - rewrite H. f_equal. clear H. induction ps; simpl; auto.
+    inversion H0; subst. rewrite H2, IHps; auto.
+  - f_equal. induction tms; simpl; auto.
+    inversion H; subst; auto. f_equal; auto.
+  - rewrite H. f_equal. clear H. induction ps; simpl; auto.
+    inversion H0; subst. rewrite H2, IHps; auto.
+Qed.
+
+(*Now prove the substitution theorem for the semantics:
+  [[t1[t2/x]]]_v = [[t1]]_(x -> t2, v)*)
+(*TODO: name with previous (and prob get rid of previous)*)
+Section SubDenot.
+
+Context {gamma: context} (gamma_valid: valid_context gamma)
+  (pd: pi_dom)(pf: pi_funpred gamma_valid pd)
+  (vt : val_typevar).
+
+(*TODO: prove that sub preserves typing*)
+
+Lemma sub_correct (t: term) (f: formula):
+  (forall (t1: term) (x: string) (ty1 ty2: vty)
+    (v: val_vars pd vt) 
+    (Hty1: term_has_type gamma t1 ty1)
+    (Hty2: term_has_type gamma t ty2)
+    (Hty3: term_has_type gamma (sub_t t1 (x, ty1) t) ty2)
+    (*The term we substitute in cannot have variables bound in
+    the original term*)
+    (Hfree: forall x, In x (tm_fv t1) ->
+      ~ In x (tm_bnd t)),
+    term_rep gamma_valid pd vt pf v (sub_t t1 (x, ty1) t) ty2 Hty3 =
+    term_rep gamma_valid pd vt pf 
+      (substi pd vt v (x, ty1) (term_rep gamma_valid pd vt pf v t1 ty1 Hty1))
+      t ty2 Hty2) /\
+  (forall (t1: term) (x: string) (ty1: vty)
+    (v: val_vars pd vt) 
+    (Hty1: term_has_type gamma t1 ty1)
+    (Hval2: formula_typed gamma f)
+    (Hval3: formula_typed gamma (sub_f t1 (x, ty1) f))
+    (*The term we substitute in cannot have variables bound in
+    the original formula*)
+    (Hfree: forall x, In x (tm_fv t1) ->
+      ~ In x (fmla_bnd f)),
+    formula_rep gamma_valid pd vt pf v (sub_f t1 (x, ty1) f) Hval3 =
+    formula_rep gamma_valid pd vt pf 
+      (substi pd vt v (x, ty1) (term_rep gamma_valid pd vt pf v t1 ty1 Hty1))
+      f Hval2).
+Proof.
+  revert t f. apply term_formula_ind; intros; simpl.
+  - destruct c; simpl_rep_full; auto;
+    unfold cast_dom_vty; simpl; do 3 f_equal;
+    apply UIP_dec; apply vty_eq_dec.
+  - (*Tvar*) 
+    simpl_rep_full.
+    revert Hty3. simpl.
+    vsym_eq (x, ty1) v; intros.
+    + unfold dom_cast. inversion Hty2; simpl in *; subst.
+      assert ((ty_var_inv Hty2) = eq_refl) by (apply UIP_dec, vty_eq_dec).
+      rewrite H. simpl. unfold var_to_dom.
+      unfold substi.
+      vsym_eq (x, ty2) (x, ty2).
+      assert (e = eq_refl) by (apply UIP_dec, vsymbol_eq_dec).
+      rewrite H0; simpl.
+      apply term_rep_irrel.
+    + simpl_rep_full.
+      unfold var_to_dom, substi. 
+      vsym_eq v (x, ty1). 
+      f_equal. f_equal. apply UIP_dec. apply vty_eq_dec.
+  - (*Tfun - need other*) admit.
+  - (*Tlet - interesting case*)
+    simpl_rep_full.
+    simpl in Hfree.
+    rewrite H with (Hty1:=Hty1)(Hty2:=proj1' (ty_let_inv Hty2)).
+    2: { intros. intro C. apply (Hfree x0); auto; rewrite in_app_iff; auto. } 
+    revert Hty3; simpl.
+    vsym_eq (x, ty1) v; intros.
+    + simpl_rep_full.
+      rewrite !substi_same.
+      apply term_rep_irrel.
+    + rewrite substi_diff; auto.
+      rewrite H0 with(Hty1:=Hty1)(Hty2:=proj2' (ty_let_inv Hty2)).
+      2: intros; intro C; apply (Hfree x0); auto; rewrite in_app_iff; auto.
+      f_equal. f_equal. apply tm_change_vv.
+      intros.
+      (*This works only because v does not appear free in t1*)
+      unfold substi. destruct (vsymbol_eq_dec x0 v); auto; subst.
+      exfalso. apply (Hfree v); auto.
+  - simpl in Hfree. simpl_rep_full. erewrite H, H0, H1; auto;
+    intros; intro C; apply (Hfree x0); auto; rewrite !in_app_iff; auto.
+  - (*Tmatch*)
+    simpl_rep_full.
+    iter_match_gen Hty2 Htm2 Hpat2 Hty2.
+    (*We need the implicit arg for map or else Coq cannot figure
+      it out*)
+    generalize dependent (proj1'
+      (@ty_match_inv _  (sub_t t1 (x, ty1) tm) _ _
+      (map (fun p : pattern * term =>
+        if in_bool vsymbol_eq_dec (x, ty1) (pat_fv (fst p))
+        then p
+        else (fst p, sub_t t1 (x, ty1) (snd p))) ps) Hty3)).
+    generalize dependent (proj1' (proj2'
+      (@ty_match_inv _  (sub_t t1 (x, ty1) tm) _ _
+      (map (fun p : pattern * term =>
+        if in_bool vsymbol_eq_dec (x, ty1) (pat_fv (fst p))
+        then p
+        else (fst p, sub_t t1 (x, ty1) (snd p))) ps) Hty3))).
+    generalize dependent (proj2' (proj2'
+      (@ty_match_inv _  (sub_t t1 (x, ty1) tm) _ _
+      (map (fun p : pattern * term =>
+        if in_bool vsymbol_eq_dec (x, ty1) (pat_fv (fst p))
+        then p
+        else (fst p, sub_t t1 (x, ty1) (snd p))) ps) Hty3))).
+    clear Hty3.
+    intros Htm3 Hpat3 Hty3; revert Htm3 Hpat3 Hty3.
+    induction ps; simpl; intros; auto.
+    destruct a as [phd thd]; simpl.
+    rewrite H with(Hty1:=Hty1)(Hty2:=Hty2). simpl.
+    2: {
+      intros; intro C; apply (Hfree x0); auto; simpl;
+      rewrite !in_app_iff; auto.
+    }
+    (*Want to say that [match_val_single] is same for both,
+      but we need to destruct [in_bool ...] to allow the dependent
+      types to match*)
+    destruct (match_val_single gamma_valid pd vt v phd (Forall_inv Hpat2)
+    (term_rep gamma_valid pd vt pf
+       (substi pd vt v0 (x, ty1) (term_rep gamma_valid pd vt pf v0 t1 ty1 Hty1)) tm v
+       Hty2)) as [newval |] eqn : Hmatch.
+    + revert Hpat3 Htm3. simpl.
+      (*Need to see if (x, ty1) is in the pat_fv of phd*)
+      destruct (in_bool_spec vsymbol_eq_dec (x, ty1) (pat_fv phd)).
+      * intros.
+        rewrite match_val_single_irrel with (Hval2:=(Forall_inv Hpat2)).
+        simpl.
+        rewrite Hmatch.
+        (*Now, we just have to reason about the two valuations*) 
+        assert (In (x, ty1) (map fst newval)). {
+          apply (match_val_single_free_var) with(x:=(x, ty1))in Hmatch.
+          apply Hmatch; auto. 
+        }
+        rewrite extend_val_substi_in; auto.
+        apply term_rep_irrel.
+        eapply match_val_single_typs.
+        apply Hmatch.
+      * (*If not in free vars, have substitution, use other IH *)
+        intros.
+        rewrite match_val_single_irrel with 
+          (Hval2:=(Forall_inv Hpat2)).
+        simpl.
+        rewrite Hmatch.
+        assert (~In (x, ty1) (map fst newval)). {
+          apply (match_val_single_free_var) with(x:=(x, ty1)) in Hmatch.
+          intro C.
+          apply Hmatch in C; auto. 
+        }
+        rewrite extend_val_substi_notin; auto.
+        2: {
+          eapply match_val_single_typs. apply Hmatch.
+        }
+        inversion H0; subst.
+        rewrite H4 with(Hty1:=Hty1)(Hty2:=Forall_inv Htm2); auto.
+        2: { intros; intro C; apply (Hfree x0); simpl; auto;
+          rewrite !in_app_iff; auto. }
+        f_equal. f_equal. 
+        (*Since we know no free vars are bound, they are not in
+          the list*)
+        apply tm_change_vv; intros.
+        rewrite extend_val_notin; auto.
+        intros Hin.
+        apply (Hfree x0); auto. simpl.
+        rewrite !in_app_iff.
+        apply (match_val_single_free_var) with(x:=x0) in Hmatch.
+        apply Hmatch in Hin. auto.
+    + (*Here, match is none, need to show equiv (easier)*)
+      revert Hpat3 Htm3. simpl.
+      (*Cases are the same (and not very interesting, just from IH)*)
+      destruct (in_bool_spec vsymbol_eq_dec (x, ty1) (pat_fv phd));
+      intros; 
+      rewrite match_val_single_irrel with 
+          (Hval2:=(Forall_inv Hpat2));
+      simpl;
+      rewrite Hmatch;
+      inversion H0; subst;
+      erewrite <- IHps with(Hpat2:=Forall_inv_tail Hpat2)
+        (Htm2:=(Forall_inv_tail Htm2))(Hty2:=Hty2); auto;
+      try (erewrite H); try reflexivity; simpl;
+      intros; intro C; apply (Hfree x0); simpl; auto;
+      rewrite !in_app_iff in *; auto;
+      destruct C; auto.
+  - (*Teps*)
+      * erewrite H. reflexivity.
+        intros; intro C; apply (Hfree x0); simpl; auto;
+        rewrite !in_app_iff; auto.
+      * simpl; intros; intro C; apply (Hfree x0); simpl; auto.
+        rewrite !in_app_iff in *; destruct C; auto.
+      * erewrite H. reflexivity.
+        
+      
+      
+      reflexivity.
+      specialize (IHps H4); rewrite IHps.
+      rewrite IHps with(Hpat2:=Forall_inv_tail Hpat2)
+        (Htm2:= (Forall_inv_tail Htm2))(Hty2:=Hty2);
+      erewrite H; auto.
+
+        
+        rewrite <- H4. with(Heq:=Heq)(Hty1:=(Forall_inv Htm1));auto.
+        f_equal. f_equal. f_equal.
+        (*Need to know that y is not bound (in the list)*)
+        unfold extend_val_with_list.
+        destruct (get_assoc_list vsymbol_eq_dec newval y) eqn : Ha; auto.
+        apply get_assoc_list_some in Ha.
+        apply match_val_single_free_var with(x:=y) in Hmatch.
+        exfalso. apply Hfree1. apply Hmatch. rewrite in_map_iff.
+        exists (y, s). split; auto.
+        eapply match_val_single_typs. apply Hmatch.
+        (*Forthis case: if var x not free in match,
+          then list does not contain it, and then
+          that we can rearrange the order of the substi
+          (basically a bigger [substi_diff]), then we apply
+          the IH (the Forall one)*)
+
+        Check extend_val_substi_in.
+
+
+
+
+
+    simpl. destruct a as [p1 t1]; simpl.
+    simpl in Hfree1.
+    rewrite !in_app_iff in Hfree1.
+    not_or Hfree.
+    destruct (match_val_single vt v p1 (Forall_inv Hpat1)
+    (term_rep vt pf
+       (substi vt v0 x (dom_cast (dom_aux pd) (f_equal (val vt) (eq_sym Heq)) (v0 y)))
+       tm v Hty1)) as [newval |] eqn : Hmatch.
+    + revert Hpat2 Htm2. simpl.
+      destruct (in_bool vsymbol_eq_dec x (pat_fv p1)) eqn : Hinp1.
+      * intros.
+        rewrite <- H with(Heq:=Heq) (Hty1:=Hty1); auto.
+        rewrite match_val_single_irrel with 
+          (Hval2:=(Forall_inv Hpat1)).
+        simpl.
+        rewrite Hmatch.
+        assert (In x (map fst newval)). {
+          apply (match_val_single_free_var) with(x:=x)in Hmatch.
+          apply Hmatch. destruct (in_bool_spec vsymbol_eq_dec x (pat_fv p1)); auto.
+          inversion Hinp1.
+        }
+       rewrite extend_val_substi_in; auto.
+       apply term_rep_irrel.
+       eapply match_val_single_typs.
+       apply Hmatch.
+      * intros.
+        rewrite <- H with(Heq:=Heq) (Hty1:=Hty1) by auto.
+        rewrite match_val_single_irrel with 
+          (Hval2:=(Forall_inv Hpat1)).
+        simpl.
+        rewrite Hmatch.
+        (*Again, use other lemma*)
+        assert (~In x (map fst newval)). {
+          apply (match_val_single_free_var) with(x:=x) in Hmatch.
+          intro C.
+          apply Hmatch in C. destruct (in_bool_spec vsymbol_eq_dec x (pat_fv p1)); auto.
+       }
+       rewrite extend_val_substi_notin; auto.
+       inversion H0; subst. 
+       rewrite <- H4 with(Heq:=Heq)(Hty1:=(Forall_inv Htm1));auto.
+       f_equal. f_equal. f_equal.
+       (*Need to know that y is not bound (in the list)*)
+       unfold extend_val_with_list.
+       destruct (get_assoc_list vsymbol_eq_dec newval y) eqn : Ha; auto.
+       apply get_assoc_list_some in Ha.
+       apply match_val_single_free_var with(x:=y) in Hmatch.
+       exfalso. apply Hfree1. apply Hmatch. rewrite in_map_iff.
+       exists (y, s). split; auto.
+       eapply match_val_single_typs. apply Hmatch.
+        (*Forthis case: if var x not free in match,
+          then list does not contain it, and then
+          that we can rearrange the order of the substi
+          (basically a bigger [substi_diff]), then we apply
+          the IH (the Forall one)*)
+    + revert Hpat2 Htm2. simpl.
+      (*Cases are the same*)
+      destruct (in_bool vsymbol_eq_dec x (pat_fv p1)) eqn : Hinp1;
+      intros;
+      rewrite <- H with(Heq:=Heq) (Hty1:=Hty1); auto;
+      rewrite match_val_single_irrel with 
+          (Hval2:=(Forall_inv Hpat1));
+      simpl;
+      rewrite Hmatch;
+      inversion H0; subst;
+      specialize (IHps H4 Hfree2);
+      rewrite IHps with(Hpat2:=Forall_inv_tail Hpat2)
+        (Htm2:= (Forall_inv_tail Htm2))(Hty2:=Hty2);
+      erewrite H; auto.
+
+
+
+    generalize dependent 
+    generalize dependent (proj1' (ty_match_inv Hty3)).
+    iter_match_gen Hty3 Htm3 Hpat3 Hty3.
+    simpl_rep_full.
+  
+
+      rewrite tm_change_vv with(t:=tm).
+      erewrite H0.
+      f_equal. f_equal.
+      apply tm_change_vv.
+      intros.
+      unfold substi.
+      destruct (vsymbol_eq_dec x0 v); subst; auto.
+      exfalso. apply (Hfree v)
+      rewrite <- H0.
+      erewrite term_rep_irrel.
+      erewrite tm_change_vv.
+      apply H0.
+      rewrite H0.
+      erewrite term_rep_irrel.
+      erewrite H0.
+
+    
+    simpl. rewrite H0. apply H0.
+      rewrite H0. 
+      apply H0.
+    (*TODO: start here - need to use fact that
+      we can change val bc agrees on free vars*)
+    
+    
+    simpl.
+
+
+      inversion Hty3; subst.
+    unfold substi.
+    
+    
+    reflexivity.
+      unfold scast.
+
+      replace ((ty_var_inv Hty2)) with eq_refl.
+
+
+  
+  simpl. unfold substi. simpl.
+  
+  
+  unfold substi. simpl.
+
+
+
+    + f_equal. f_equal. f_equal. apply UIP_dec.
+    
+    term_
+    )
+
+Lemma sub_correct (t: term) (f: formula) :
+(forall (x y: vsymbol) (Heq: snd x = snd y) 
+  (v: val_vars pd vt) (ty: vty) 
+  (Hty1: term_has_type gamma t ty)
+  (Hty2: term_has_type gamma (sub_var_t x y t) ty)
+  (Hfree: ~In y (tm_bnd t)),
+  term_rep vt pf (substi vt v x 
+  (dom_cast _ (f_equal (val vt) (eq_sym Heq))
+    (v y))) t ty Hty1 =
+  term_rep vt pf v (sub_var_t x y t) ty Hty2) /\
+(forall (x y: vsymbol) (Heq: snd x = snd y) 
+  (v: val_vars pd vt)
+  (Hval1: formula_typed gamma f)
+  (Hval2: formula_typed gamma (sub_var_f x y f))
+  (Hfree: ~In y (fmla_bnd f)),
+  formula_rep vt pf (substi vt v x 
+  (dom_cast _ (f_equal (val vt) (eq_sym Heq))
+    (v y))) f Hval1 =
+  formula_rep vt pf v (sub_var_f x y f) Hval2).
